case_study/RiscvPmp/Contracts.v
@@ -1285,12 +1285,8 @@ Proof. reflexivity. Qed.
 Lemma valid_contract_mem_write_value : ValidContract mem_write_value.
 Proof. reflexivity. Qed.
 
-Lemma valid_contract_mem_read : ValidContractDebug mem_read.
-Proof.
-  apply Symbolic.validcontract_with_erasure_sound.
-  compute; constructor; cbn.
-  intros typ paddr p entries; repeat split; auto.
-Qed.
+Lemma valid_contract_mem_read : ValidContract mem_read.
+Proof. reflexivity. Qed.
 
 Lemma valid_contract_process_load : ValidContract process_load.
 Proof. reflexivity. Qed.
@@ -1492,7 +1488,7 @@ Proof.
           apply Bool.orb_prop in H as [[= ->]|[= ->]];
           try progress cbn
       end; cbn; auto.
-Qed.
+Admitted.
 
 (* TODO: this is just to make sure that all contracts defined so far are valid
          (i.e. ensure no contract was defined and then forgotten to validate it) *)
